Type dependant on alphabet

src/DFA.lean
@@ -2,8 +2,9 @@ import data.fintype.basic
 
 universes u v
 
-structure DFA := 
-(alphabet : Type u) 
+variable {α : Type u}
+
+structure DFA (alphabet : Type u) :=
 [alphabet_fintype : fintype alphabet]
 (state : Type v)
 [state_fintype : fintype state]
@@ -13,10 +14,10 @@ structure DFA :=
 
 namespace DFA
 
-def eval (M : DFA) : list M.alphabet → M.state :=
+def eval (M : DFA α) : list α → M.state :=
 list.foldl M.step M.start
 
-def accepts (M : DFA) (s : list M.alphabet) : Prop :=
+def accepts (M : DFA α) (s : list α) : Prop :=
 M.eval s ∈ M.accept_states
 
 end DFA
